src/util/list/nil.lean
@@ -1,0 +1,12 @@
+theorem nothing_mem_nil {t: Type} {xs: list t}: (∀ (x: t), x ∉ xs) ↔ xs = [] :=
+begin
+  split,
+  intro h,
+  induction xs,
+  refl,
+  exfalso,
+  exact h xs_hd (or.inl rfl),
+  intro h,
+  rw h,
+  exact list.not_mem_nil,
+end
